FormalUrchin/proofs/mirlight_proofs.lean
@@ -1,0 +1,88 @@
+import FormalUrchin.mirlight
+
+open mir
+
+theorem readWordSeq_concat (mem : Mem) (addr : Word) (head : MemValue) (tail : List MemValue) :
+  ReadWordSeq mem addr 1 = [head] →
+  ReadWordSeq mem (addr + 1) tail.length = tail →
+  ReadWordSeq mem addr (tail.length + 1) = head :: tail := by
+    intros h_head h_tail
+    have h_read_head : ReadWordSeq mem addr 1 = [head] →
+      mem.mMap.find? addr = some head  := by
+      cases heq : Lean.AssocList.find? addr mem.mMap
+      case some v' =>
+        intros h_read_head1
+        simp [ReadWordSeq] at h_read_head1
+        rw [heq] at h_read_head1
+        --injection h_head with h_eq
+        simp at h_read_head1
+        congr
+      case none =>
+        intros h_read_head1
+        simp [ReadWordSeq] at h_read_head1
+        rw [heq] at h_read_head1
+        contradiction
+    have h_some_head := h_read_head h_head
+    simp [ReadWordSeq]
+    rw [h_some_head]
+    rw [h_tail]
+    simp
+
+theorem readWordSeq_returns_sequence_of_bytes (mem : Mem) (addr : Word) (values : List MemValue) :
+  (∀ i, (h: i < values.length) → mem.mMap.find? (addr + i) = some (values.get ⟨i, h⟩)) →
+  ReadWordSeq mem addr values.length = values := by
+  intros h_memhasvalues
+  induction values generalizing addr
+  case nil =>
+    simp [ReadWordSeq]
+  case cons head tail ih =>
+    simp [ReadWordSeq]
+    have h_head_eq : mem.mMap.find? addr = some head := h_memhasvalues 0 (by simp)
+    have h_tail_eq : ∀ i, (h: i < tail.length) → mem.mMap.find? (addr + i + 1) = some (tail.get ⟨i, h⟩) := by
+      intros i h_i
+      specialize h_memhasvalues (i + 1)
+      simp at h_memhasvalues
+      simp
+      apply h_memhasvalues h_i
+    have h_head_read_ok : ReadWordSeq mem addr 1 = [head] := by
+      simp [ReadWordSeq]
+      simp [h_head_eq]
+    have h_tail_read_ok : ReadWordSeq mem (addr + 1)
+      tail.length = tail := by
+      apply ih
+      intros i h_i
+      specialize h_memhasvalues (i + 1)
+      simp at h_memhasvalues
+      rw [Nat.add_assoc,Nat.add_comm 1 i,]
+      exact h_memhasvalues h_i
+    have h_concat := readWordSeq_concat mem addr head tail h_head_read_ok h_tail_read_ok
+    exact h_concat
+
+
+@[simp]
+theorem step_pc_stays_same_iff_halt2
+    {bb: BB} {pc : PC} {prog : Prog} {env : Env} {mem : Mem} {ap : accessperm.AccessPerms}
+    {stmt_list : List Stmt}
+    (h_bb : prog.find? bb = some stmt_list)
+    (h_stmt: pc < stmt_list.length):
+      (stmt_list.get ⟨pc, h_stmt⟩ = Stmt.Halt) ↔
+    Eval2 (bb, pc, prog, env, mem, ap) (bb, pc, prog, env, mem, ap) := by
+  apply Iff.intro
+  { intros h_stmt_eq
+    apply Eval2.HaltRel
+    exact h_bb
+    exact h_stmt_eq
+  }
+  {
+    intros h
+    cases h
+    case HaltRel s1 s2 s3 s4 =>
+     -- Unify stmt_list and s1
+      have : stmt_list = s1 := by
+        rw [s4] at h_bb
+        injection h_bb with h_eq
+        symm
+        exact h_eq
+      subst this
+      exact s3
+}
